So llist2 was a good way to learn but not so useful

src/llist.lean
@@ -2,28 +2,24 @@ import tactic
 
 inductive llist (V : Type) : Type | P : V -> llist | L : V -> llist -> llist
 
-@[ext] structure llist2 (V : Type) := (head : V) (tail : list V)
-
 namespace llist section
-    parameters {V W : Type} (adj : V -> V -> Prop)
-
-    def fold (f : V -> W) (g : V -> W -> W) : llist V -> W | (P v) := f v | (L v l) := g v (fold l)
+    variables {V W : Type} (adj : V -> V -> Prop) (f : V -> W)
 
     def mem (x) : llist V -> Prop | (P v) := x = v | (L v l) := x = v ∨ mem l
     instance : has_mem V (llist V) := ⟨mem⟩
 
-    @[simp] def to_list          : llist V -> list V  | (P v) := [v]       | (L v l) := v :: to_list l
-    @[simp] def size             : llist V -> nat     | (P _) := 0         | (L v l) := (size l) + 1
-    @[simp] def head             : llist V -> V       | (P v) := v         | (L v l) := v
-    @[simp] def tail             : llist V -> list V  | (P v) := []        | (L v l) := l.head :: tail l
-    @[simp] def init             : llist V -> list V  | (P v) := []        | (L v l) := v :: init l
-    @[simp] def last             : llist V -> V       | (P v) := v         | (L v l) := last l
-    @[simp] def inside           : llist V -> list V  | (P v) := []        | (L v l) := init l
-    @[simp] def is_path          : llist V -> Prop    | (P v) := true      | (L v l) := adj v l.head ∧ is_path l
-    @[simp] def append   (x : V) : llist V -> llist V | (P v) := L v (P x) | (L v l) := L v (append l)
-    @[simp] def rev              : llist V -> llist V | (P v) := (P v)     | (L v l) := append v (rev l)
-    @[simp] def nodup            : llist V -> Prop    | (P v) := true      | (L v l) := v ∉ l ∧ nodup l
-    @[simp] def map (f : V -> W) : llist V -> llist W | (P v) := P (f v)   | (L v l) := L (f v) (map l)
+    @[simp] def to_list        : llist V -> list V  | (P v) := [v]       | (L v l) := v :: to_list l
+    @[simp] def size           : llist V -> nat     | (P _) := 0         | (L v l) := (size l) + 1
+    @[simp] def head           : llist V -> V       | (P v) := v         | (L v l) := v
+    @[simp] def tail           : llist V -> list V  | (P v) := []        | (L v l) := l.head :: tail l
+    @[simp] def init           : llist V -> list V  | (P v) := []        | (L v l) := v :: init l
+    @[simp] def last           : llist V -> V       | (P v) := v         | (L v l) := last l
+    @[simp] def inside         : llist V -> list V  | (P v) := []        | (L v l) := init l
+    @[simp] def is_path        : llist V -> Prop    | (P v) := true      | (L v l) := adj v l.head ∧ is_path l
+    @[simp] def append (x : V) : llist V -> llist V | (P v) := L v (P x) | (L v l) := L v (append l)
+    @[simp] def rev            : llist V -> llist V | (P v) := (P v)     | (L v l) := append v (rev l)
+    @[simp] def nodup          : llist V -> Prop    | (P v) := true      | (L v l) := v ∉ l ∧ nodup l
+    @[simp] def map            : llist V -> llist W | (P v) := P (f v)   | (L v l) := L (f v) (map l)
 
     @[simp] def concat : llist V -> llist V -> llist V | (P _) l' := l' | (L v l) l' := L v (concat l l')
     
@@ -58,7 +54,7 @@ namespace llist section
     @[simp] lemma mem_singleton : x ∈ P y <-> x = y := iff.rfl
     @[simp] lemma mem_cons : x ∈ L v l <-> x = v ∨ x ∈ l := iff.rfl
 
-    @[simp] lemma is_path_concat (h : compat l l') : is_path (concat l l') <-> is_path l ∧ is_path l'
+    @[simp] lemma is_path_concat (h : compat l l') : is_path adj (concat l l') <-> is_path adj l ∧ is_path adj l'
         := by { induction l, tauto, simp at h, finish [l_ih h,head_concat h] }
 
     @[simp] lemma mem_append : w ∈ append v l <-> w = v ∨ w ∈ l
@@ -82,7 +78,7 @@ namespace llist section
     @[simp] lemma nodup_rev : nodup (rev l) <-> nodup l
         := by { induction l, simp, simp [l_ih] }
 
-    @[simp] lemma append_is_path : is_path (append v l) <-> adj (last l) v ∧ is_path l
+    @[simp] lemma append_is_path : is_path adj (append v l) <-> adj (last l) v ∧ is_path adj l
         := by { induction l; finish }
 
     lemma init_append : init (append x l) = to_list l
@@ -115,28 +111,24 @@ namespace llist section
     @[simp] lemma inside_rev : inside (rev l) = (inside l).reverse
         := by { cases l, refl, simp }
 
-    @[simp] lemma is_path_rev (h : symmetric adj) : is_path (rev l) <-> is_path l
+    @[simp] lemma is_path_rev (h : symmetric adj) : is_path adj (rev l) <-> is_path adj l
         := by { induction l, trivial, simp [l_ih], exact and_congr ⟨@h _ _, @h _ _⟩ iff.rfl }
--- HERE
+
     @[simp] lemma mem_concat (h : compat l l') : x ∈ concat l l' <-> x ∈ l ∨ x ∈ l'
         := by { induction l,
-            { rw [concat,mem_singleton], refine ⟨or.inr, _⟩, 
-                intro h1, cases h1, convert head_mem, rwa h1, exact h1 }, 
-            { rw [concat,mem_cons,l_ih h,mem_cons,or.assoc] } }
+            { simp at ⊢ h, subst h, cases l', simp, simp, rw [<-or_assoc,or_self] },
+            { simp at ⊢ h, simp [l_ih h,or_assoc] } }
 
-    @[simp] lemma concat_nil      (h : last l = w) : concat l (P w)           = l
-        := by { rw <-h, clear h, induction l, refl, { rw [concat,last,l_ih] } }
+    @[simp] lemma concat_nil (h : last l = w) : concat l (P w) = l
+        := by { subst h, induction l, refl, simpa }
 
-    @[simp] lemma concat_nil2                      : concat (P w) l           = l
-        := rfl
+    @[simp] lemma concat_size : size (concat l l') = size l + size l'
+        := by { induction l, simp, simp [l_ih] }
 
-    @[simp] lemma concat_size                      : size (concat l l')       = size l + size l'
-        := by { induction l; rw [concat,size], { norm_num }, { rw [l_ih,size], norm_num } }
-
-    lemma         concat_assoc                     : concat (concat l l') l'' = concat l (concat l' l'')
+    lemma concat_assoc : concat (concat l l') l'' = concat l (concat l' l'')
         := by { induction l; rw [concat,concat], rw [l_ih,concat] }
 
-    lemma         concat_nodup   (h : compat l l') : nodup (concat l l')    <-> nodup l ∧ nodup l' ∧ (∀ x, x ∈ l ∧ x ∈ l' -> x = head l')
+    lemma concat_nodup (h : compat l l') : nodup (concat l l') <-> nodup l ∧ nodup l' ∧ (∀ x, x ∈ l ∧ x ∈ l' -> x = head l')
         := by { induction l with v v l hr; rw [concat,nodup],
             { split, { intro, refine ⟨trivial,a,_⟩, intros x h1, rw mem_singleton at h1, rwa h1.1 }, tauto },
             { rw [nodup,hr h], rw [compat,last] at h, split,
@@ -148,74 +140,64 @@ namespace llist section
                     { intro h5, have h6 := h4 v ⟨(or.inl rfl),h5⟩, subst h6, rw <-h at h1, exact (h1 last_mem) },
                     { rintros x ⟨h5,h6⟩, exact h4 x ⟨(or.inr h5),h6⟩ } } } }
 
-    lemma         mem_iff             (h : l = l') : x ∈ l                  <-> x ∈ l'
-        := by { rw h }
-
-    lemma         mem_init        (h : x ∈ init l) : x ∈ l
+    lemma mem_init (h : x ∈ init l) : x ∈ l
         := by { induction l, cases h, cases h, exact or.inl h, exact or.inr (l_ih h) }
 
-    lemma         mem_head_init'                   : v ∈ init (L v l)
-        := by { rw [init], left, refl }
+    lemma mem_head_init (h : 0 < size l) : head l ∈ init l
+        := by { cases l, cases h, left, refl }
 
-    lemma         mem_head_init   (h : 0 < size l) : head l ∈ init l
-        := by { cases l, cases h, exact mem_head_init' }
+    lemma mem_last_tail (h : 0 < size l) : last l ∈ tail l
+        := by { cases l with v v l, cases h, induction l, simp, right, exact l_ih nat.succ_pos' }
 
-    lemma         mem_last_tail   (h : 0 < size l) : last l ∈ tail l
-        := by { cases l, cases h, clear h, rw [last,tail], induction l_a_1,
-            { left, refl }, { rw [last,head,tail], right, assumption } }
-
-    lemma         mem_tail        (h : x ∈ tail l) : x ∈ l
+    lemma mem_tail (h : x ∈ tail l) : x ∈ l
         := by { cases l, cases h, rw [tail,head_tail,mem_list] at h, right, assumption }
 
-    lemma         mem_init_last                    : x ∈ l                  <-> x ∈ init l ∨ x = last l
+    lemma mem_init_last : x ∈ l <-> x ∈ init l ∨ x = last l
         := by { split,
             { intro, induction l, { right, assumption }, { cases a, { left, left, exact a },
                 cases l_ih a, { left, right, assumption }, { right, rwa last } } },
             { intro, cases a, exact mem_init a, convert last_mem } }
 
-    lemma         mem_head_tail                    : x ∈ l                  <-> x = head l ∨ x ∈ tail l
+    lemma mem_head_tail : x ∈ l <-> x = head l ∨ x ∈ tail l
         := by { cases l, { rw [mem_singleton,head,tail], convert (or_false _).symm },
             { rw [head,tail,head_tail,mem_list,mem_cons] } }
 
-    lemma         mem_init_inside'                 : x ∈ init (L v l)       <-> x = v ∨ x ∈ inside (L v l)
-        := by { rw [init,inside,list.mem_cons_iff] }
-
-    lemma         mem_init_inside (h : 0 < size l) : x ∈ init l             <-> x = head l ∨ x ∈ inside l
+    lemma mem_init_inside (h : 0 < size l) : x ∈ init l <-> x = head l ∨ x ∈ inside l
         := by { rw [<-(head_inside h),list.mem_cons_iff] }
 
-    lemma         mem_tail_inside'                 : x ∈ tail (L v l)       <-> x ∈ inside (L v l) ∨ x = last l
+    lemma mem_tail_inside' : x ∈ tail (L v l) <-> x ∈ inside (L v l) ∨ x = last l
         := by { rw [inside,<-mem_init_last,tail,mem_head_tail], trivial }
 
-    lemma         mem_tail_inside (h : 0 < size l) : x ∈ tail l             <-> x ∈ inside l ∨ x = last l
+    lemma mem_tail_inside (h : 0 < size l) : x ∈ tail l <-> x ∈ inside l ∨ x = last l
         := by { rw [<-(inside_last h),list.mem_append_eq,list.mem_singleton] }
 
-    lemma         nodup_mem_head     (h : nodup l) : head l ∉ tail l
+    lemma nodup_mem_head (h : nodup l) : head l ∉ tail l
         := by { cases l, { rw [tail,list.mem_nil_iff], trivial }, 
             { rw [head,tail,head_tail,mem_list], exact h.1 } }
 
-    lemma         nodup_mem_last     (h : nodup l) : last l ∉ init l
+    lemma nodup_mem_last (h : nodup l) : last l ∉ init l
         := by { induction l, { rw [init,list.mem_nil_iff], trivial }, 
             { rw [last,init,list.mem_cons_iff], push_neg, split,
                 { intro, apply h.1, convert last_mem, exact a.symm },
                 { exact l_ih h.2 } } }
 
-    lemma         rev_compat                       : compat l l' <-> compat l'.rev l.rev
+    lemma rev_compat : compat l l' <-> compat l'.rev l.rev
         := by { rw [compat,compat,last_rev,head_rev,eq_comm] }
 
-    lemma         concat_append                    : append v (concat l l')  = concat l (append v l')
+    lemma concat_append : append v (concat l l')  = concat l (append v l')
         := by { induction l; rw [concat,concat], rw [append,l_ih] }
 
-    lemma         rev_concat     (h : compat l l') : rev (concat l l')       = concat (rev l') (rev l)
+    lemma rev_concat (h : compat l l') : rev (concat l l') = concat (rev l') (rev l)
         := by { induction l,
             { rw [concat,rev,concat_nil], rw [last_rev], exact h.symm },
             { rw [concat,rev,l_ih h,concat_append,rev] } }
 
-    lemma         nodup_init         (h : nodup l) : list.nodup (init l)
+    lemma nodup_init (h : nodup l) : list.nodup (init l)
         := by { induction l, { exact list.pairwise.nil }, 
             { rw [init,list.nodup,list.pairwise_cons], refine ⟨_,l_ih h.2⟩, 
                 intros a h1 h2, replace h := h.1, rw h2 at h, exact h (mem_init h1) } }
 
-    lemma         nodup_of_init : list.nodup (init l) -> last l ∉ init l -> nodup l
+    lemma nodup_of_init : list.nodup (init l) -> last l ∉ init l -> nodup l
         := by { induction l, { intros, trivial },
             { rw [init,last,nodup,list.nodup_cons,list.mem_cons_iff], push_neg, 
                 rintros ⟨h1,h2⟩ ⟨h3,h4⟩, refine ⟨_,l_ih h2 h4⟩,
@@ -226,10 +208,6 @@ namespace llist section
 
     lemma size_rev : size l.rev = size l
         := by { induction l, refl, rw [rev,size_append,l_ih,size], }
-end end llist
-
-namespace llist section
-    parameters {V W : Type}
 
     lemma size_map {f : V -> W} {l : llist V} : size (map f l) = size l
         := by { induction l, refl, rw [map,size,l_ih,size] }
@@ -240,312 +218,6 @@ namespace llist section
     lemma last_map {f : V -> W} {l : llist V} : last (map f l) = f (last l)
         := by { induction l, refl, rwa [map,last,last] }
 end end llist
-
-namespace llist2 section
-    variables {V W : Type} (f : V -> W) (adj : V -> V -> Prop) {C : llist2 V -> Prop}
-
-    @[simp] def cons : V -> llist2 V -> llist2 V | u ⟨x,l⟩ := ⟨u,x::l⟩
-
-    lemma cases_on' (l) (h0 : ∀ {x}, C ⟨x,[]⟩) (h1 : ∀ {x} (y ys), C (cons x ⟨y,ys⟩)) : C l 
-        := cases_on l $ λ x l, list.cases_on l h0 h1
-
-    def rec' {C : llist2 V → Sort*} (h0 : Π a, C ⟨a,[]⟩) (h1 : Π {a l}, C l → C (cons a l)) (l) : C l
-        := cases_on l $ λ x l, list.rec h0 (λ y l hr x, h1 (hr y)) l x
-
-    def rec'' := @rec' V (λ _, W)
-
-    lemma induction_on (l) (h0 : ∀ x, C ⟨x,[]⟩) (h1 : ∀ (x l) (hr : C l), C (cons x l)) : C l 
-        := rec' h0 h1 l
-
-    def fold (f : V -> W) (g : V -> W -> W) (l : llist2 V) : W
-        := rec'' f (λ a l, g a) l
-
-    def fold' (f : V -> W) (g : V -> V -> W -> W) (l : llist2 V) : W
-        := cases_on l $ λ x l, list.rec f (λ y ys φ x, g x y (φ y)) l x
-
-    def fold'' (f : V -> W) (g : V -> llist2 V -> W -> W) (l : llist2 V) : W
-        := cases_on l $ λ x l, list.rec f (λ y ys φ x, g x ⟨y,ys⟩ (φ y)) l x
-
-    @[simp] lemma fold_init   {f g x}      : @fold   V W f g ⟨x,[]⟩    = f x                            := rfl
-    @[simp] lemma fold'_init  {f g x}      : @fold'  V W f g ⟨x,[]⟩    = f x                            := rfl
-    @[simp] lemma fold''_init {f g x}      : @fold'' V W f g ⟨x,[]⟩    = f x                            := rfl
-    @[simp] lemma fold_step   {f g x y ys} : @fold   V W f g ⟨x,y::ys⟩ = g x (fold f g ⟨y,ys⟩)          := rfl
-    @[simp] lemma fold'_step  {f g x y ys} : @fold'  V W f g ⟨x,y::ys⟩ = g x y (fold' f g ⟨y,ys⟩)       := rfl
-    @[simp] lemma fold''_step {f g x y ys} : @fold'' V W f g ⟨x,y::ys⟩ = g x ⟨y,ys⟩ (fold'' f g ⟨y,ys⟩) := rfl
-
-    def mem : V -> llist2 V -> Prop | u ⟨x,l⟩ := u = x ∨ u ∈ l
-    def mem' (v : V) : llist2 V -> Prop := fold (eq v) (or ∘ eq v)
-    instance : has_mem V (llist2 V) := ⟨mem⟩
-
-    def size    :             llist2 V -> nat      |       ⟨x,l⟩   := l.length
-    def to_list :             llist2 V -> list V   |       ⟨x,l⟩   := x :: l
-    def append' :        V -> llist2 V -> llist2 V |     u ⟨x,l⟩   := ⟨x, l ++ [u]⟩
-    def concat  : llist2 V -> llist2 V -> llist2 V | ⟨x,l⟩ ⟨x',l'⟩ := ⟨x, l ++ l'⟩
-    def map     : (V -> W) -> llist2 V -> llist2 W |     f ⟨x,l⟩   := ⟨f x, list.map f l⟩
-    
-    def size'       : llist2 V -> ℕ                    := fold   (λ _, 0)            (λ _, nat.succ)
-    def append  (v) : llist2 V -> llist2 V             := fold   (λ x, ⟨x,[v]⟩)      cons
-    def reverse     : llist2 V -> llist2 V             := fold   (λ x, ⟨x,[]⟩)       append
-    def last        : llist2 V -> V                    := fold   id                  (λ _, id)
-    def init        : llist2 V -> list V               := fold   (λ _, [])           list.cons
-    def concat'     : llist2 V -> llist2 V -> llist2 V := fold   (λ x y, ⟨x,y.tail⟩) ((∘)∘cons)
-    def concat_'    : llist2 V -> llist2 V -> llist2 V := fold   (λ _, id)           ((∘)∘cons)
-    def is_path     : llist2 V -> Prop                 := fold'  (λ _, true)         (λ x, and ∘ adj x)
-    def nodup       : llist2 V -> Prop                 := fold'' (λ _, true)         (λ x, and ∘ not ∘ (∈) x)
-    
-    def map' : llist2 V -> llist2 W := fold (λ x, ⟨f x, []⟩) (cons ∘ f)
-
-    def inside  : llist2 V -> list V   | ⟨x,[]⟩ := []     | ⟨x,y::l⟩ := init ⟨y,l⟩
-
-    @[simp] def compat (l₁ l₂ : llist2 V) := last l₁ = head l₂
-
-    variables {x y v w : V} {l l' l'' : llist2 V} {xs ys zs : list V}
-
-    @[simp] lemma mem_cons     : x ∈ cons v l           <-> x = v ∨ x ∈ l                := by { cases l, refl }
-    @[simp] lemma head_cons    : head (cons v l)         =  v                            := by { cases l, refl }
-    @[simp] lemma last_cons    : last (cons v l)         =  last l                       := by { cases l, refl }
-    @[simp] lemma append_cons  : append w (cons v l)     =  cons v (append w l)          := by { cases l, refl }
-    @[simp] lemma reverse_cons : reverse (cons v l)      =  append v (reverse l)         := by { cases l, refl }
-    @[simp] lemma init_cons    : init (cons v l)         =  v :: init l                  := by { cases l, refl }
-    @[simp] lemma is_path_cons : is_path adj (cons v l) <-> adj v l.head ∧ is_path adj l := by { cases l, refl }
-    @[simp] lemma to_list_cons : to_list (cons v l)      =  v :: to_list l               := by { cases l, refl }
-    @[simp] lemma inside_cons  : inside (cons v l)       =  init l                       := by { cases l, refl }
-    @[simp] lemma tail_cons    : tail (cons v l)         =  l.head :: l.tail             := by { cases l, refl }
-    @[simp] lemma concat'_cons : concat' (cons v l) l'   =  cons v (concat' l l')        := by { cases l, refl }
-    @[simp] lemma size'_cons   : size' (cons v l)        =  size' l + 1                  := by { cases l, refl }
-    @[simp] lemma nodup_cons   : nodup (cons v l)       <-> v ∉ l ∧ nodup l              := by { cases l, refl }
-    @[simp] lemma map'_cons    : map' f (cons v l)        =  cons (f v) (map' f l)       := by { cases l, refl }
-
-    @[simp] lemma mem_cons'     : v ∈ llist2.mk x (y::ys) <-> v = x ∨ v ∈ llist2.mk y ys             := iff.rfl
-    @[simp] lemma last_cons'    : last ⟨x,y::ys⟩           = last ⟨y,ys⟩                             := rfl
-    @[simp] lemma append_cons'  : append w ⟨x,y::ys⟩       = cons x (append w ⟨y,ys⟩)                := rfl
-    @[simp] lemma reverse_cons' : reverse ⟨x,y::ys⟩        = append x (reverse ⟨y,ys⟩)               := rfl
-    @[simp] lemma init_cons'    : init ⟨x,y::ys⟩           = x :: init ⟨y,ys⟩                        := rfl
-    @[simp] lemma nodup_cons'   : nodup ⟨x,y::ys⟩         <-> x ∉ (⟨y,ys⟩ : llist2 V) ∧ nodup ⟨y,ys⟩ := iff.rfl
-
-    @[simp] lemma head_concat : head (concat l l') = head l
-        := by { cases l, cases l', refl }
-
-    @[simp] lemma head_concat' : head (concat' l l') = head l
-        := by { rcases l with ⟨x,_|⟨y,ys⟩⟩, refl, simp [concat'] }
-
-    @[simp] lemma concat_point : concat' l ⟨x,[]⟩ = l
-        := by { apply induction_on l; intros, refl, simp [hr] }
-
-    lemma concat_point' (h : x = l'.head) : concat' ⟨x,[]⟩ l' = l'
-        := by { cases l', rw [concat',fold_init,h] }
-
-    @[simp] lemma last_concat (h : compat l l') : last (concat' l l') = last l'
-        := by { revert h, apply induction_on l; intros,
-            { rw [concat_point'], exact h },
-            { simp, rw [compat,last_cons] at h, apply hr h } }
-
-    @[simp] lemma head_append : head (append v l) = head l
-        := by { apply induction_on l; intros, refl, simp }
-
-    @[simp] lemma last_append : last (append v l) = v
-        := by { apply induction_on l; intros, refl, simpa }
-
-    @[simp] lemma rev_append : reverse (append v l) = cons v (reverse l)
-        := by { apply induction_on l; intros, refl, simp [hr] }
-
-    @[simp] lemma rev_head : head (reverse l) = last l
-        := by { apply induction_on l; intros, refl, simpa }
-
-    @[simp] lemma rev_last : last (reverse l) = head l
-        := by { apply cases_on' l; intros, refl, rw [reverse_cons,last_append], refl }
-
-    @[simp] lemma rev_rev : reverse (reverse l) = l
-        := by { apply induction_on l; intros, refl, simp [hr] }
-
-    lemma mem_iff : x ∈ l <-> x = head l ∨ x ∈ tail l
-        := by { cases l, trivial }
-
-    @[simp] lemma mem_singleton : x ∈ (⟨y,[]⟩ : llist2 V) <-> x = y
-        := by { simp [mem_iff] }
-
-    @[simp] lemma is_path_concat (h : compat l l') : is_path adj (concat' l l') <-> is_path adj l ∧ is_path adj l'
-        := by { revert h, apply induction_on l; intros,
-            { simp [compat,last] at h, subst h, rw [concat_point'], simp [is_path] },
-            { rw [compat,last_cons] at h, simp [hr h], finish } }
-
-    @[simp] lemma mem_append : w ∈ append v l <-> w = v ∨ w ∈ l
-        := by { apply induction_on l; intros, simp [append,or.comm], 
-            rw [append_cons,mem_cons,mem_cons,hr], finish }
-
-    @[simp] lemma mem_rev : v ∈ reverse l <-> v ∈ l
-        := by { apply induction_on l; intros, refl, simp [hr] }
-
-    @[simp] lemma mem_head : head l ∈ l
-        := by { cases l, left, refl }
-
-    @[simp] lemma mem_last : last l ∈ l
-        := by { apply induction_on l; intros; finish }
-
-    @[simp] lemma mem_list : x ∈ to_list l <-> x ∈ l
-        := by { cases l, trivial }
-
-    @[simp] lemma append_nodup : nodup (append x l) <-> x ∉ l ∧ nodup l
-        := by { apply induction_on l; intros,
-            { simp [append,nodup,mem], exact ne_comm },
-            { rw [append_cons,nodup_cons,hr,mem_append,nodup_cons], finish } }
-
-    @[simp] lemma rev_nodup : nodup (reverse l) <-> nodup l
-        := by { apply induction_on l; intros, trivial, simp [hr] }
-
-    @[simp] lemma append_is_path : is_path adj (append v l) <-> adj (last l) v ∧ is_path adj l
-        := by { apply induction_on l; intros, { simp [append,is_path,last] }, 
-            { simp [hr], finish } }
-
-    @[simp] lemma init_append : init (append x l) = to_list l
-        := by { apply induction_on l; intros, refl, { simp [hr] } }
-
-    @[simp] lemma init_last : init l ++ [last l] = to_list l
-        := by { apply induction_on l; intros, refl, simpa }
-
-    @[simp] lemma head_inside' : v :: inside (cons v l) = init (cons v l)
-        := by { apply induction_on l; intros, refl, simp }
-
-    @[simp] lemma head_inside (h : l.tail ≠ []) : head l :: inside l = init l
-        := by { revert h, apply cases_on' l; intros, contradiction, refl }
-
-    @[simp] lemma inside_last' : inside (cons v l) ++ [last (cons v l)] = tail (cons v l)
-        := by { cases l, exact init_last }
-
-    @[simp] lemma inside_last (h : l.tail ≠ []) : inside l ++ [last l] = tail l
-        := by { cases l with x l, cases l, contradiction, exact init_last }
-
-    @[simp] lemma init_inside (h : l.tail ≠ []) : init l = (head l) :: inside l
-        := by { revert h, apply induction_on l; intros, contradiction, simp }
-
-    lemma tail_cons' : tail (cons v l) = to_list l
-        := by { apply cases_on' l; intros, refl, simp [to_list] }
-
-    @[simp] lemma inside_append : inside (append x l) = tail l
-        := by { apply induction_on l; intros, refl, simp [tail_cons'] }
-
-    @[simp] lemma tail_append : (append x l).tail = tail l ++ [x]
-        := by { apply induction_on l; intros, refl, simpa }
-
-    @[simp] lemma tail_rev : tail (reverse l) = list.reverse (init l)
-        := by { apply induction_on l; intros, refl, simp [hr] }
-
-    @[simp] lemma inside_rev : inside (reverse l) = list.reverse (inside l)
-        := by { apply cases_on' l; intros, refl, 
-            rw [reverse_cons,inside_append,tail_rev], refl } 
-
-    @[simp] lemma is_path_rev (h : symmetric adj) : is_path adj (reverse l) <-> is_path adj l
-        := by { apply induction_on l; intros, trivial, 
-            simp [hr], exact and_congr ⟨@h _ _, @h _ _⟩ iff.rfl }
-
-    @[simp] lemma mem_concat (h : compat l l') : x ∈ concat l l' <-> x ∈ l ∨ x ∈ l'
-        := by { replace h : head l' ∈ l, by { rw compat at h, rw <-h, exact mem_last },
-            have : x ∈ concat l l' <-> x ∈ l ∨ x ∈ l'.tail, 
-                by { cases l, cases l', rw [concat,mem_iff], simp [or.assoc,mem_iff] }, 
-            rw [this,@mem_iff _ x l'], split; finish }
-
-    @[simp] lemma concat_nil (h : last l = w) : concat l ⟨w,[]⟩ = l
-        := by { revert h, apply cases_on' l; intros, refl, simp [cons,concat] }
-
-    @[simp] lemma concat_nil' (h : w = head l) : concat ⟨w,[]⟩ l = l
-        := by { subst h, cases l, refl }
-
-    @[simp] lemma concat_size : size (concat l l') = size l + size l'
-        := by { cases l, cases l', simp [concat,size] }
-
-    lemma concat_assoc : concat (concat l l') l'' = concat l (concat l' l'')
-        := by { cases l, cases l', cases l'', simp [concat] }
-
-    -- lemma concat_nodup (h : compat l l') : nodup (concat l l')
-    --             <-> nodup l ∧ nodup l' ∧ (∀ v, v ∈ l ∧ v ∈ l' -> v = head l')
-    --     := by { revert h, apply induction_on l; intros,
-    --         { simp [compat,last] at h, subst h, rw [concat_nil' rfl], simp [nodup] },
-    --         { cases l, cases l', simp [concat] at *, rw [nodup_cons', hr h, nodup], clear hr, 
-    --             simp [mem_iff], push_neg, split,
-    --             { rintros ⟨⟨h1,h2,h3⟩,h4,h5,h6,h7⟩, refine ⟨⟨⟨h1,h2⟩,h4⟩,h5,_⟩, 
-    --                 intros v h8 h9, cases h9, assumption,
-    --                 cases h8, subst h8, contradiction,
-    --                 cases h8, subst h8, apply h6, exact or.inr h9,
-    --                 apply h7 v h8, exact or.inr h9 },
-    --             { rintros ⟨⟨⟨h1,h2⟩,h3⟩,h4,h5⟩, refine ⟨⟨h1,h2,_⟩,h3,h4,_,_⟩,
-    --                 { intro h7, have h6 := h5 x (or.inl rfl) (or.inr h7), subst h6,
-    --                     revert h4 h7, cases l'_tail; intros, cases h7, 
-    --                     simp at h4, apply h4.1, simp at h7, exact h7 },
-    --                 { exact h5 y (or.inr (or.inl rfl)) },
-    --                 { intros x, exact h5 x ∘ or.inr ∘ or.inr } } } }
-
-    lemma mem_init (h : x ∈ init l) : x ∈ l
-        := by { revert h, apply induction_on l; intros, cases h,
-            simp at h, simp, cases h, exact or.inl h, exact or.inr (hr h) }
-
-    lemma mem_head_init (h : l.tail ≠ []) : head l ∈ init l
-        := by { revert h, apply cases_on' l; intros, simp at h, contradiction, left, refl }
-
-    lemma mem_last_tail (h : l.tail ≠ []) : last l ∈ tail l
-        := by { revert h, apply induction_on l; intros, simp at h, contradiction,
-            simp, revert hr, apply cases_on' l_1; intros, { left, refl }, { right, apply hr, trivial } }
-
-    lemma mem_tail : x ∈ tail l -> x ∈ l
-        := by { rw mem_iff, exact or.inr }
-
-    lemma mem_init_last : x ∈ l <-> x ∈ init l ∨ x = last l
-        := by { apply induction_on l; intros, simp [init,last], simp [hr], finish }
-
-    lemma mem_init_inside' : x ∈ init (cons v l) <-> x = v ∨ x ∈ inside (cons v l)
-        := by { cases l, rw [init_cons,cons,inside,list.mem_cons_iff] }
-
-    lemma mem_init_inside (h : l.tail ≠ []) : x ∈ init l <-> x = head l ∨ x ∈ inside l
-        := by { rw [<-(head_inside h),list.mem_cons_iff] }
-
-    lemma mem_tail_inside' : x ∈ tail (cons v l) <-> x ∈ inside (cons v l) ∨ x = last l
-        := by { cases l with u l, rw [cons,inside,<-mem_init_last], simp [mem_iff] }
-
-    lemma mem_tail_inside (h : l.tail ≠ []) : x ∈ tail l <-> x ∈ inside l ∨ x = last l
-        := by { rw [<-(inside_last h),list.mem_append_eq,list.mem_singleton] }
-
-    lemma nodup_mem_head (h : nodup l) : head l ∉ tail l
-        := by { revert h, apply cases_on' l; intros, simp, exact h.1 }
-
-    lemma nodup_mem_last (h : nodup l) : last l ∉ init l
-        := by { revert h, apply induction_on l; intros,
-            { simp [last,init] },
-            { simp at h, simp, push_neg, split, exact λ hh, (hh.symm ▸ h.1) mem_last, exact hr h.2 } }
-
-    lemma rev_compat : compat l l' <-> compat l'.reverse l.reverse
-        := by { rw [compat,compat,rev_last,rev_head,eq_comm] }
-
-    lemma concat_append : append v (concat' l l')  = concat' l (append v l')
-        := by { apply induction_on l; intros,
-            { rw [concat',fold_init], apply llist2.ext, rw head_append, simp },
-            { simp [hr] } }
-
-    lemma rev_concat (h : compat l l') : reverse (concat' l l') = concat' (reverse l') (reverse l)
-        := by { revert h, apply induction_on l; intros,
-            { simp [last] at h, rw [concat_point' h,reverse,fold_init,concat_point] },
-            { simp, rw [hr], rw [concat_append], rw [compat,last_cons] at h, exact h } }
-
-    lemma nodup_init (h : nodup l) : list.nodup (init l)
-        := by { revert h, apply induction_on l; intros, simp [init],
-            simp at ⊢ h, split, exact h.1 ∘ mem_init, exact hr h.2 }
-
-    lemma nodup_of_init : list.nodup (init l) -> last l ∉ init l -> nodup l
-        := by { apply induction_on l; intros, trivial,
-            simp at ⊢ a a_1, push_neg at a_1, split,
-                { intro h, cases mem_init_last.mp h, exact a.1 h_1, exact a_1.1 h_1.symm },
-                { exact hr a.2 a_1.2 } }
-
-    lemma head_map {f : V -> W} {l : llist2 V} : head (map f l) = f (head l)
-        := by { cases l, refl }
-
-    lemma last_map {f : V -> W} {l : llist2 V} : last (map' f l) = f (last l)
-        := by { apply induction_on l; intros, refl, simpa }
-
-    @[simp] lemma size_append : size' (append v l) = size' l + 1
-        := by { apply induction_on l; intros, refl, simp [hr] }
-
-    lemma size_reverse : size' l.reverse = size' l
-        := by { apply induction_on l; intros, refl, simpa }
-end end llist2
 
 @[ext] structure llist' (V : Type) (x y : V) := (l : llist V) (hx : l.head = x) (hy : l.last = y)
 instance {V : Type} {x y : V} : has_coe (llist' V x y) (llist V) := ⟨llist'.l⟩
@@ -559,11 +231,10 @@ namespace llist' section open llist
 
     @[simp] lemma reduce {l hx hy} : (⟨l,hx,hy⟩ : llist' V x y).l = l := rfl
 
-    @[simp] lemma mem_simp {v l hx hy} : v ∈ (⟨l,hx,hy⟩ : llist' V x y) <-> v ∈ l
-        := by { trivial }
+    @[simp] lemma mem_simp {v l hx hy} : v ∈ (⟨l,hx,hy⟩ : llist' V x y) <-> v ∈ l := iff.rfl
 
-    def P    (v : V)                    : llist' V v v := ⟨P v,     rfl, rfl⟩
-    def cons (v : V) (l : llist' V x y) : llist' V v y := ⟨L v l.l, rfl, l.hy⟩
+    def P    (v : V)                    : llist' V v v := ⟨P v,   rfl, rfl⟩
+    def cons (v : V) (l : llist' V x y) : llist' V v y := ⟨L v l, rfl, l.hy⟩
 
     lemma compat {l : llist' V x y} {l' : llist' V y z} : llist.compat l.l l'.l 
         := eq.trans l.hy l'.hx.symm
@@ -574,34 +245,3 @@ namespace llist' section open llist
     @[simp] lemma concat_P {l : llist' V x y} : concat l (P y) = l
         := by { ext, exact llist.concat_nil l.hy }
 end end llist'
-
-structure llist2' (V : Type) (x y : V) := (l : llist2 V) (hx : l.head = x) (hy : l.last = y)
-instance {V : Type} {x y : V} : has_coe (llist2' V x y) (llist2 V) := ⟨llist2'.l⟩
-
-namespace llist2' section open llist2
-    parameters {V : Type} (adj : V -> V -> Prop)
-    variables {x y z : V}
-
-    def mem (v : V) (l : llist2' V x y) := v ∈ l.l
-    instance has_mem : has_mem V (llist2' V x y) := ⟨mem⟩
-
-    @[ext] lemma ext {l l' : llist2' V x y} : l.l = l'.l -> l = l'
-        := by { cases l, cases l', simp }
-
-    @[simp] lemma reduce {l hx hy} : (⟨l,hx,hy⟩ : llist2' V x y).l = l := rfl
-
-    @[simp] lemma mem_simp {v l hx hy} : v ∈ (⟨l,hx,hy⟩ : llist2' V x y) <-> v ∈ l
-        := by { trivial }
-
-    def P    (v : V)                     : llist2' V v v := ⟨⟨v,[]⟩, rfl, rfl⟩
-    def cons (v : V) (l : llist2' V x y) : llist2' V v y := ⟨cons v l.l, head_cons, by { rw last_cons, exact l.hy } ⟩
-
-    lemma compat {l : llist2' V x y} {l' : llist2' V y z} : llist2.compat l.l l'.l 
-        := eq.trans l.hy l'.hx.symm
-
-    def concat {x y z : V} (l : llist2' V x y) (l' : llist2' V y z) : llist2' V x z
-        := ⟨llist2.concat' l l', eq.trans head_concat' l.hx, eq.trans (last_concat compat) l'.hy⟩
-
-    @[simp] lemma concat_P {l : llist2' V x y} : concat l (P y) = l
-        := by { apply ext, apply concat_point }
-end end llist2'
